src/3d/Binding.fsti
@@ -36,3 +36,7 @@ val parser_kind_nz (env:global_env) (id:ident) : ML (option bool)
 val map_opt (f:'a -> ML 'b) (o:option 'a) : ML (option 'b)
 val size_of_integral_typ (_:env) (_:typ) (_:range) : ML int
 val bind_decls (p:list decl) : ML (list decl & global_env)
+val next_field_num (enclosing_struct:ident)
+                   (field_name:ident)
+                   (_:env)
+    : ML field_num
